Fix broken MVCC proofs

external/Goose/github_com/mit_pdos/go_mvcc/config.v
@@ -7,7 +7,7 @@ Local Coercion Var' s: expr := Var s.
 
 Definition N_TXN_SITES : expr := #64.
 
-Definition N_IDX_BUCKET : expr := #2048.
+Definition N_IDX_BUCKET : expr := #8192.
 
 Definition TID_SENTINEL : expr := #18446744073709551615.
 
